I2MP/Examples/Factorial.v
@@ -1,0 +1,10 @@
+Require Import Common.Definitions.
+Require Import Common.Values.
+Require Import Transitional.
+Require Import Source.Examples.Factorial.
+
+Definition fuel := 1000%nat.
+Definition to_run := compile_and_run_from_source_ex factorial fuel.
+
+Set Warnings "-extraction-reserved-identifier".
+Extraction "/tmp/run_mp_compiled_factorial.ml" to_run.
