MicroPolicies/Transitional.v
@@ -1,0 +1,812 @@
+Require Import CompCert.Events.
+Require Import CompCert.Smallstep.
+Require Import CompCert.Behaviors.
+Require Import Common.Definitions.
+Require Import Common.Memory.
+Require Import Common.Traces.
+(* TL TODO: Ariths Export is a pain *)
+
+From mathcomp Require Import ssreflect ssrfun eqtype seq.
+From extructures Require Import fmap fset.
+
+Require Import Intermediate.Machine.
+Require Import Intermediate.GlobalEnv.
+Require Import MicroPolicies.LRC.
+Require Import Tmp.
+Require Import Linearize.
+
+Require Import Lib.Extra.
+Require Import Lib.Monads.
+Import MonadNotations.
+Open Scope monad_scope.
+Import Intermediate.
+
+Require Import Source.Language.
+
+Definition proc_label : Set := Component.id * Procedure.id.
+
+Definition plabel : Set := label * option proc_label.
+
+Definition label_of (pl : plabel) : label := let (n,_) := pl in n.
+
+Variant instr :=
+| TrNop : instr
+| TrLabel : plabel -> instr
+(* register operations *)
+| TrConst : imvalue -> register -> instr
+| TrMov : register -> register -> instr
+| TrBinOp : binop -> register -> register -> register -> instr
+(* memory operations *)
+| TrLoad : register -> register -> instr
+| TrStore : register -> register -> instr
+| TrAlloc : register -> register -> instr
+(* conditional and unconditional jumps *)
+| TrBnz : register -> label -> instr
+| TrJump : register -> instr
+| TrJalNat : label -> instr
+| TrJalProc : proc_label -> instr
+(* termination *)
+| TrHalt : instr.
+
+
+
+Record mem_tag : Type := MTag
+  { vtag : value_tag;
+    entry : option (Procedure.id * seq Component.id) }.
+
+
+
+
+Definition code := NMap (seq (instr * mem_tag)).
+Definition def_mem_tag (c : Component.id) := MTag Other None.
+
+
+Record compiler_env :=
+  { program : Intermediate.program ;
+    make_label : Component.id -> Procedure.id -> label ;
+  }.
+
+
+Definition instr_to_transitional (cenv : compiler_env)
+           (c : Component.id) (i : Machine.instr) : (instr * mem_tag) :=
+  match i with
+  | ICall c' P => if beq_nat c c' then  ((TrJalNat (make_label cenv c' P)), def_mem_tag c)
+    else ((TrJalProc (c',P)), def_mem_tag c)
+  | IReturn => ((TrJump R_RA), def_mem_tag c)
+  | INop => (TrNop, def_mem_tag c)
+  | ILabel l =>  (TrLabel (l,None), def_mem_tag c)
+  | IConst v r =>  (TrConst v r, def_mem_tag c)
+  | IMov r r' => (TrMov r r', def_mem_tag c)
+  | IBinOp op r r' r'' => (TrBinOp op r r' r'', def_mem_tag c)
+  | ILoad r r' => (TrLoad r r', def_mem_tag c)
+  | IStore r r' => (TrStore r r', def_mem_tag c)
+  | IAlloc r r' => (TrAlloc r r', def_mem_tag c)
+  | IBnz r l => (TrBnz r l, def_mem_tag c)
+  | IJump r => (TrJump r, def_mem_tag c)
+  | IJal l => (TrJalNat l, def_mem_tag c)
+  | IHalt => (TrHalt, def_mem_tag c)
+  end.
+
+
+Definition executing (cde : code) (pc : Pointer.t) (i : instr) (tg : mem_tag) (c : Component.id)  : Prop := 
+    exists C_code,
+    Pointer.component pc = c /\
+    cde c = Some C_code /\
+    (Pointer.offset pc >= 0) % Z /\
+    nth_error C_code (Z.to_nat (Pointer.offset pc)) = Some (i,tg).
+
+
+(* Inductive F := FallThrough | Jumped.
+
+Definition pc_tag : Type := F * Component.id.
+
+
+Inductive check_pc : pc_tag -> mem_tag -> Prop := 
+ | PcFall : forall c mt, color mt = c -> check_pc (FallThrough,c) mt
+ | PcJump : forall c mt pid l, entry mt = Some (pid,l) -> check_comp_belongs c l -> check_pc (Jumped,c) mt. *)
+
+
+Inductive pc_tag : Type := Level : nat -> pc_tag.
+
+Definition level (pct : pc_tag) : nat := match pct with Level n => n end.
+
+Definition inc_pc_tag (pct : pc_tag) : pc_tag := Level (level pct + 1).
+
+(* Here: rather do an option thing? *)
+Definition dec_pc_tag (pct : pc_tag) : pc_tag := Level (level pct - 1).
+
+(* Definition level (pct : pc_tag) : nat := match pct with (n,c) => n end. *)
+
+Fixpoint check_comp_belongs (c : Component.id) (l : seq Component.id) : Prop := match l with 
+ | nil => False
+ | c' :: l' => c = c' \/ check_comp_belongs c l'
+end.
+
+Fixpoint check_comp_belongs_b (c : Component.id) (l : seq Component.id) : bool := match l with 
+ | nil => false
+ | c' :: l' => if Nat.eqb c c' then true else check_comp_belongs_b c l'
+end.
+
+
+(* 
+Inductive check_pc_samec : mem_tag -> mem_tag -> Prop := 
+ | PcFall : forall c ti tni, color ti = c -> color tni = c -> check_pc_samec ti tni.
+
+Inductive check_pc_callret : mem_tag -> mem_tag -> Prop := 
+ | PcJump : forall c ti tni pid l, color ti = c -> entry tni = Some (pid,l) -> 
+check_comp_belongs c l -> check_pc_callret ti tni. *)
+
+
+Definition state : Type := list Pointer.t * Memory.t * Intermediate.Register.t * Pointer.t * pc_tag.
+
+Definition stackless : Type := Memory.t * Intermediate.Register.t * Pointer.t * pc_tag.
+
+
+Fixpoint find_label (cd : seq (instr * mem_tag)) (l : label) : option Z :=
+  let fix aux c o :=
+      match c with
+      | [] => None
+      | (TrLabel l',_) :: c' =>
+        if Nat.eqb l (label_of l') then
+          Some o
+        else
+          aux c' (1 + o)%Z
+      | _ :: c' =>
+        aux c' (1 + o)%Z
+      end
+  in aux cd 0%Z.
+
+
+Definition find_label_in_comp (cde : code) (c : Component.id) (l : label) : option Pointer.t :=
+  match cde c with
+  | Some C_comp =>
+      match find_label C_comp l with
+      | Some offset => Some (c, 0, offset)
+      | None => None
+      end
+  | None => None
+end.
+
+Fixpoint find_label_in_code_helper
+         (cde : code) (comps: list (Component.id * (seq (instr * mem_tag))))
+         (l: label) : option Pointer.t :=
+  match comps with
+   | [] => None
+   | (comp_id,comp_code) :: comps' => find_label_in_comp cde comp_id l
+  end.
+
+Definition find_label_in_code (cde : code) (l : label) : option Pointer.t :=
+  find_label_in_code_helper cde (elementsm cde) l.
+
+
+Fixpoint find_plabel (cd : seq (instr * mem_tag)) (c : Component.id) (p : Procedure.id) : option Z :=
+  let fix aux cd o :=
+      match cd with
+      | [] => None
+      | (TrLabel (_,Some (c',p')),_) :: cd' =>
+        if Nat.eqb c c' && Nat.eqb p p' then
+          Some o
+        else
+          aux cd' (1 + o)%Z
+      | _ :: cd' =>
+        aux cd' (1 + o)%Z
+      end
+  in aux cd 0%Z.
+
+
+Definition find_plabel_in_code (cde : code) (c : Component.id) (p : Procedure.id) : option Pointer.t :=
+  match cde c with
+  | Some C_comp =>
+      match find_plabel C_comp c p with
+      | Some offset => Some (c, 0, offset)
+      | None => None
+      end
+  | None => None
+end.
+
+
+
+
+(*      match find_label cde l with
+      | Some offset => Some (Pointer.component pc, Pointer.block pc, offset)
+      | None => None
+      end.
+
+
+Fixpoint find_label_in_component_helper
+         G (procs: list (Block.id * code))
+         (pc: Pointer.t) (l: label) : option Pointer.t :=
+  match procs with
+  | [] => None
+  | (p_block,p_code) :: procs' =>
+    match find_label_in_procedure G (Pointer.component pc, p_block, 0%Z) l with
+    | None => find_label_in_component_helper G procs' pc l
+    | Some ptr => Some ptr
+    end
+  end.
+
+Definition find_label_in_component G (pc : Pointer.t) (l : label) : option Pointer.t :=
+  match getm (genv_procedures G) (Pointer.component pc) with
+  | Some C_procs =>
+    find_label_in_component_helper G (elementsm C_procs) pc l
+  | None => None *)
+
+
+
+
+Inductive check_pc : code -> Pointer.t -> mem_tag -> Prop :=
+| PcFall : forall cde pc tg i tni c, 
+    executing cde (Pointer.inc pc) i tni c ->
+    (* color tg = c -> *) check_pc cde pc tg.
+
+
+Inductive check_pc_jump : code -> mem_tag -> Pointer.t -> Component.id -> Prop :=
+ |PcJump : forall cde tg pc' i tni c c0,
+    executing cde (pc') i tni c ->
+    Pointer.component pc' = c0 -> check_pc_jump cde tg pc' c0.
+
+Inductive check_pc_call : Component.id -> mem_tag -> Procedure.id -> Prop := 
+ | PcCall : forall c tni pid l, (* color ti = c ->  *)
+  entry tni = Some (pid,l) -> 
+  check_comp_belongs c l -> check_pc_call c tni pid.
+
+
+(* missing stuff *)
+Inductive check_pc_ret : Component.id -> mem_tag -> Prop := 
+ | PcRet : forall c tni pid l, (* color ti = c ->  *)
+  entry tni = Some (pid,l) -> 
+  check_comp_belongs c l -> check_pc_ret c tni.
+
+
+(*** !IMPORTANT: PROTECT Return Adress registers with tags in a 'linear' way,
+                 so that they can't be copied ***)
+(* make the code separated  by compartments in the compilation *)
+(* well-formedness & interfaces *)
+(*step for return *)
+(* where is return adress stored?*)
+(* TODO Add Jal for (c,pid) type (TrJalProc), but intra compartment ?? 
+todo? (in order to reduce UB), allow TrJalNat to different components *)
+
+Inductive step (cde : code) : state -> trace -> state -> Prop :=
+| Nop: forall st mem regs pc tg c pct,
+    executing cde pc TrNop tg c ->
+    check_pc cde pc tg ->
+    step cde (st, mem, regs, pc, pct) E0
+           (st, mem, regs, Pointer.inc pc, pct)
+
+| Label: forall st mem regs pc tg c pct l,
+    executing cde pc (TrLabel l) tg c ->
+    check_pc cde pc tg ->
+    step cde (st, mem, regs, pc, pct) E0
+           (st, mem, regs, Pointer.inc pc, pct)
+
+| Const: forall st mem regs regs' pc tg c pct r v,
+    executing cde pc (TrConst  v r) tg c ->
+    check_pc cde pc tg ->
+    Register.set r (imm_to_val v) regs = regs' ->
+    step cde (st, mem, regs, pc, pct) E0
+           (st, mem, regs', Pointer.inc pc, pct)
+
+| Mov: forall st mem regs regs' pc tg c pct r1 r2,
+    executing cde pc (TrMov r1 r2) tg c ->
+    check_pc cde pc tg ->
+    Register.set r2 (Register.get r1 regs) regs = regs' ->
+    step cde (st, mem, regs, pc, pct) E0
+           (st, mem, regs', Pointer.inc pc, pct)
+
+| BinOp: forall st mem regs regs' pc tg c pct r1 r2 r3 op,
+    executing cde pc (TrBinOp op r1 r2 r3) tg c ->
+    check_pc cde pc tg ->
+    let result := eval_binop op (Register.get r1 regs) (Register.get r2 regs) in
+    Register.set r3 result regs = regs' ->
+    step cde (st, mem, regs, pc, pct) E0
+           (st, mem, regs', Pointer.inc pc, pct)
+
+| Load: forall st mem regs regs' pc tg c pct r1 r2 ptr v,
+    executing cde pc (TrLoad r1 r2) tg c ->
+    check_pc cde pc tg ->
+    Register.get r1 regs = Ptr ptr ->
+    Pointer.component ptr = c ->
+    Memory.load mem ptr = Some v ->
+    Register.set r2 v regs = regs' ->
+    step cde (st, mem, regs, pc, pct) E0
+           (st, mem, regs', Pointer.inc pc, pct)
+
+| Store: forall st mem mem' regs pc tg c pct ptr r1 r2,
+    executing cde pc (TrStore r1 r2) tg c ->
+    check_pc cde pc tg ->
+    Register.get r1 regs = Ptr ptr ->
+    Pointer.component ptr =  c ->
+    Memory.store mem ptr (Register.get r2 regs) = Some mem' ->
+    step cde (st, mem, regs, pc, pct) E0
+           (st, mem', regs, Pointer.inc pc, pct)
+
+| Jal: forall st mem regs regs' pc tg c pct pc' l,
+    executing cde pc (TrJalNat l) tg c ->
+(*   check_pc cde pc tg ->*)
+(*    find_label_in_component G pc l = Some pc' -> *)
+    find_label_in_code cde l = Some pc' ->
+    Register.set R_RA (Ptr (Pointer.inc pc)) regs = regs' ->
+    check_pc_jump cde tg pc' c ->
+    step cde (st, mem, regs, pc, pct) E0
+           (st, mem, regs', pc', pct)
+
+| Jump: forall st mem regs pc tg c pct pc' r,
+    executing cde pc (TrJump r) tg c ->
+(*    check_pc cde pc tg ->*)
+    Register.get r regs = Ptr pc' ->
+(*    Pointer.component pc' = Pointer.component pc -> *)
+    check_pc_jump cde tg pc' c ->
+    step cde (st, mem, regs, pc, pct) E0
+           (st, mem, regs, pc', pct)
+
+| BnzNZ: forall st mem regs pc tg c pct pc' r l val,
+    executing cde pc (TrBnz r l) tg c ->
+(*    check_pc cde pc tg ->*)
+    Register.get r regs = Int val ->
+    (val <> 0) % Z ->
+    find_label_in_code cde l = Some pc' ->
+    check_pc_jump cde tg pc' c ->
+    step cde (st, mem, regs, pc, pct) E0
+           (st, mem, regs, pc', pct)
+
+| BnzZ: forall st mem regs pc tg c pct r l,
+    executing cde pc (TrBnz r l) tg c ->
+    check_pc cde pc tg ->
+    Register.get r regs = Int 0 ->
+    step cde (st, mem, regs, pc, pct) E0
+           (st, mem, regs, Pointer.inc pc, pct)
+
+| Alloc: forall st mem mem' regs regs' pc tg c pct rsize rptr size ptr,
+    executing cde pc (TrAlloc rptr rsize) tg c ->
+    check_pc cde pc tg ->
+    Register.get rsize regs = Int size ->
+    (size > 0) % Z ->
+    Memory.alloc mem c (Z.to_nat size) = Some (mem', ptr) ->
+    Register.set rptr (Ptr ptr) regs = regs' ->
+    step cde (st, mem, regs, pc, pct) E0
+           (st, mem', regs', Pointer.inc pc, pct)
+
+| Call: forall st mem regs regs' pc tg c pct pc' i tni c' pid call_arg,
+    executing cde pc (TrJalProc (c',pid)) tg c ->
+(*   check_pc cde pc tg ->*)
+(*    find_label_in_component G pc l = Some pc' -> *)
+    find_plabel_in_code cde c' pid = Some pc' ->
+    executing cde pc' i tni c' ->
+    c <> c' ->
+    check_pc_call c tni pid ->
+    Register.set R_RA (Ptr (Pointer.inc pc)) regs = regs' ->
+    Register.get R_COM regs = Int call_arg ->
+    step cde (st, mem, regs, pc, pct) [ECall c pid call_arg c']
+           (Pointer.inc pc :: st, mem, Register.invalidate regs', pc', inc_pc_tag pct).
+
+
+
+Import MonadNotations.
+Open Scope monad_scope.
+
+
+
+Definition eval_step (cde: code) (s: stackless) : option (trace * stackless) :=
+  let '(mem, regs, pc, pct) := s in
+  (* fetch the next instruction to execute *)
+  if (Pointer.offset pc <? 0) % Z then
+    None
+  else
+    do C_code <- cde (Pointer.component pc);
+    do (instr,tag) <- nth_error C_code (Z.to_nat (Pointer.offset pc));
+    match instr with
+    | TrLabel _ =>
+      ret (E0, (mem, regs, Pointer.inc pc, pct))
+    | TrNop =>
+      ret (E0, (mem, regs, Pointer.inc pc, pct))
+    | TrConst v r =>
+      let regs' := Register.set r (imm_to_val v) regs in
+      ret (E0, (mem, regs', Pointer.inc pc, pct))
+    | TrMov r1 r2 =>
+      let regs' := Register.set r2 (Register.get r1 regs) regs in
+      ret (E0, (mem, regs', Pointer.inc pc, pct))
+    | TrBinOp op r1 r2 r3 =>
+      let result := eval_binop op (Register.get r1 regs) (Register.get r2 regs) in
+      let regs' := Register.set r3 result regs in
+      ret (E0, (mem, regs', Pointer.inc pc, pct))
+    | TrLoad r1 r2 =>
+      match Register.get r1 regs with
+      | Ptr ptr =>
+        if Component.eqb (Pointer.component ptr) (Pointer.component pc) then
+          do v <- Memory.load mem ptr;
+          let regs' := Register.set r2 v regs in
+          ret (E0, (mem, regs', Pointer.inc pc, pct))
+        else
+          None
+      | _ => None
+      end
+    | TrStore r1 r2 =>
+      match Register.get r1 regs with
+      | Ptr ptr =>
+        if Component.eqb (Pointer.component ptr) (Pointer.component pc) then
+          do mem' <- Memory.store mem ptr (Register.get r2 regs);
+          ret (E0, (mem', regs, Pointer.inc pc, pct))
+        else
+          None
+      | _ => None
+      end
+    | TrAlloc rptr rsize =>
+      match Register.get rsize regs with
+      | Int size =>
+        if (size <=? 0) % Z then
+          None
+        else
+          do (mem', ptr) <- Memory.alloc mem (Pointer.component pc) (Z.to_nat size);
+          let regs' := Register.set rptr (Ptr ptr) regs in
+          ret (E0, (mem', regs', Pointer.inc pc, pct))
+      | _ => None
+      end
+    | TrJump r =>
+      match Register.get r regs with
+      | Ptr pc' =>
+        if Component.eqb (Pointer.component pc') (Pointer.component pc) then
+          ret (E0, (mem, regs, pc', pct))
+        else
+         if (Pointer.offset pc' <? 0) % Z then
+            None
+         else
+            do C_code' <- cde (Pointer.component pc');
+            do (ni,tni) <- nth_error C_code' (Z.to_nat (Pointer.offset pc'));
+            match Register.get R_COM regs with
+            | Int rcomval =>
+              let t := [ERet (Pointer.component pc) rcomval (Pointer.component pc')] in
+              ret (t, (mem, Register.invalidate regs, pc', dec_pc_tag pct))
+            | _ => None
+            end
+            (* MISSING HERE : ENFORCEMENT ABOUT LEVEL OF RETURN AND RA (should be same level) *)
+      | _ => None
+      end
+    | TrBnz r l =>
+      match Register.get r regs with
+      | Int 0 =>
+        ret (E0, (mem, regs, Pointer.inc pc, pct))
+      | Int val =>
+        do pc' <- find_label_in_code cde l;
+        ret (E0, (mem, regs, pc', pct))
+      | _ => None
+      end
+    | TrJalNat l =>
+      do pc' <- find_label_in_code cde l;
+      let regs' := Register.set R_RA (Ptr (Pointer.inc pc)) regs in
+      ret (E0, (mem, regs', pc', pct))
+    | TrJalProc (c',pid) =>
+      match find_plabel_in_code cde c' pid with 
+      | Some pc' => 
+        if Component.eqb (Pointer.component pc') (Pointer.component pc) then
+          ret (E0, (mem, regs, pc', pct))
+        else 
+         if (Pointer.offset pc' <? 0) % Z then
+            None
+         else
+            do C_code' <- cde (Pointer.component pc');
+            do (ni,tni) <- nth_error C_code' (Z.to_nat (Pointer.offset pc'));
+            match entry tni with
+             | Some (pid',lc) => 
+               if Procedure.eqb pid pid' then 
+                if check_comp_belongs_b (Pointer.component pc) lc then
+                  match Register.get R_COM regs with
+                  | Int rcomval =>
+                      let regs' := Register.set R_RA (Ptr (Pointer.inc pc)) regs in
+                      let t := [ECall (Pointer.component pc) pid rcomval (Pointer.component pc')] in
+                      ret (t, (mem, Register.invalidate regs', pc', inc_pc_tag pct))
+                  | _ => None
+                  end
+                else None
+               else None
+             | _ => None
+            end
+      | None => None
+      end
+    | _ => None
+end.
+
+
+Fixpoint execN (n: nat) (cde: code) (st: stackless) : option Z :=
+  match n with
+  | O => None
+  | S n' =>
+    match eval_step cde st with
+    | None =>
+      let '(_, regs, _, _) := st in
+      match Register.get R_COM regs with
+      | Int i => Some i
+      | _ => None
+      end
+    | Some (_, st') => execN n' cde st'
+    end
+  end.
+
+
+
+Definition head_tag (cenv : compiler_env) (c : Component.id) (p : Procedure.id) : mem_tag :=
+  let I := Intermediate.prog_interface (program cenv) in
+  let allowed_call_by (c' : Component.id) :=
+      Option.default false (do i <- getm I c ;
+                            do i' <- getm I c' ;
+                            Some ((p \in Component.export i) && ((c, p) \in Component.import i')))
+  in {| vtag := Other ;
+        entry := Some (p, filter allowed_call_by (domm I)) |}.
+
+Print getm.
+
+Definition linearize_proc (cenv : compiler_env)
+           (c : Component.id) (p : Procedure.id) : seq (instr * mem_tag) :=
+  let code := Option.default [:: ] (do map <- getm (Intermediate.prog_procedures (program cenv)) c;
+                                    getm map p)
+  in ((TrLabel (make_label cenv c p, Some (c,p))), head_tag cenv c p) :: (map (instr_to_transitional cenv c) code).
+
+Definition linearize_component (cenv : compiler_env) (c : Component.id) : seq (instr * mem_tag) :=
+  let procs : seq Procedure.id :=
+      Option.default fset0 (do map <- getm (Intermediate.prog_procedures (program cenv)) c;
+                            Some (domm map)) in
+  flatten (map (linearize_proc cenv c) procs).
+
+Check mapm.
+Print NMap.
+
+Fixpoint compile_component_list {T} cenv (l : list (Component.id * T)) :=
+ match l with 
+  | [] => []
+  | (c,_) :: cs => (c,linearize_component cenv c) :: compile_component_list cenv cs
+end.
+
+Definition intermediate_to_transitional (cenv : compiler_env) : code := 
+mkfmap (compile_component_list cenv (elementsm (Intermediate.prog_procedures (program cenv)))).
+
+
+
+
+Definition pre_linearize (p : Intermediate.program) : code :=
+  let lmax := max_label p in
+  let pmax := max_proc_id p in
+  let cenv := {| program := p ;
+                 make_label := (fun c p => lmax + c * pmax + p) |} in
+ intermediate_to_transitional cenv.
+
+(* Record program : Type := mkProg
+    prog_code : code;
+    prog_buffers : NMap {fmap Block.id -> nat + seq value};
+    prog_main : bool } *)
+
+
+Definition run_transitional cd fuel p :=
+    let '(mem, _, entrypoints) := prepare_procedures_initial_memory p in
+    let regs := Register.init in
+    match (find_plabel_in_code cd Component.main Procedure.main) with
+    | Some pc =>
+      execN fuel cd (mem,regs, pc, Level 0)
+    | None => None
+end.
+
+Definition compile_run fuel (p : Intermediate.program) :=
+  run_transitional (pre_linearize p) fuel p.
+
+Close Scope monad_scope.
+
+
+Require Import Compiler.
+
+Definition compile_and_run_from_source := 
+fun (p : Source.program) (fuel : nat) =>
+match Compiler.compile_program p with
+| Some compiled_p =>
+    match compile_run fuel compiled_p with
+    | Some n => Some n
+    | None => None
+    end
+| None => None
+end.
+
+Require Export Extraction.Definitions.
+
+Definition compile_and_run_from_source_ex := 
+fun (p : Source.program) (fuel : nat) =>
+match Compiler.compile_program p with
+| Some compiled_p =>
+    match compile_run fuel compiled_p with
+    | Some n => print_ocaml_int (z2int n)
+    | None => print_error ocaml_int_1
+    end
+| None => print_error ocaml_int_0
+end.
+
+
+(* Require Import Source.Examples.Identity.
+
+Eval compute in compile_and_run_from_source_ex identity 10.*)
+
+
+
+
+
+(*version for extraction : 
+Definition compile_and_run_from_source := 
+fun (p : Source.program) (fuel : nat) =>
+match Compiler.compile_program p with
+| Some compiled_p =>
+    match compile_run fuel compiled_p with
+    | Some n => print_ocaml_int (z2int n)
+    | None => print_error ocaml_int_1
+    end
+| None => print_error ocaml_int_0
+end.  *)
+
+
+
+(*
+Theorem eval_step_complete:
+  forall G st t st',
+    step G st t st' -> eval_step G st = Some (t, st').
+
+
+Theorem eval_step_sound:
+  forall G st t st',
+    eval_step G st = Some (t, st') -> step G st t st'. *)
+
+
+
+
+
+(*** BELOW : OLD COMPILATION PROCEDURE (WORKED WITH SINGLE CODE BLOCK, NOT 
+NECESSARY TO ADAPT DIRECTLY FROM THERE ***)
+
+(* Definition head_tag (cenv : compiler_env) (c : Component.id) (p : Procedure.id) : mem_tag :=
+  let I := Intermediate.prog_interface (program cenv) in
+  let allowed_call_by (c' : Component.id) :=
+      Option.default false (do i <- getm I c ;
+                            do i' <- getm I c' ;
+                            Some ((p \in Component.export i) && ((c, p) \in Component.import i')))
+  in {| vtag := Other ;
+        color := c ;
+        entry := Some (p, filter allowed_call_by (domm I)) |}.
+
+
+Definition linearize_proc (cenv : compiler_env)
+           (c : Component.id) (p : Procedure.id) : code :=
+  let code := Option.default [:: ] (do map <- getm (Intermediate.prog_procedures (program cenv)) c;
+                                    getm map p)
+  in (inr (ILabel (make_label cenv c p)), head_tag cenv c p) :: flatten (map (linearize_instr cenv c) code).
+
+Definition linearize_component (cenv : compiler_env) (c : Component.id) : code :=
+  let procs : seq Procedure.id :=
+      Option.default fset0 (do map <- getm (Intermediate.prog_procedures (program cenv)) c;
+                            Some (domm map)) in
+  flatten (map (linearize_proc cenv c) procs).
+
+Definition linearize_code (cenv : compiler_env) : code :=
+  let main_code :=
+      [:: (inr (IJal (make_label cenv Component.main Procedure.main)), def_mem_tag Component.main) ; (inr IHalt, def_mem_tag Component.main)] in
+
+  let components : seq Component.id := domm (Intermediate.prog_procedures (program cenv)) in
+  main_code ++ flatten (map (linearize_component cenv) components).
+
+
+Notation bufs := {fmap (nat * nat * nat) -> (value * mem_tag)}.
+
+Definition linearize_buf (cenv : compiler_env) (c : Component.id) (b : Block.id) : seq (value * mem_tag) :=
+  Option.default [::] (do map <- getm (Intermediate.prog_buffers (program cenv)) c ;
+                       do block <- getm map b ;
+                       Some match block with
+                            | inl n => repeat (Undef, def_mem_tag c) n
+                            | inr l => [seq (x, def_mem_tag c) | x <- l]
+                            end).
+
+Definition linearize_bufs (cenv : compiler_env) : bufs :=
+  let bufs' : NMap (NMap (NMap (value * mem_tag))) :=
+      mapim (fun c map => mapim (fun b _ => fmap_of_seq (linearize_buf cenv c b)) map)
+            (Intermediate.prog_buffers (program cenv))
+  in Tmp.mapk (fun c => match c with (x, (y, z)) => (x, y, z) end)
+              (uncurrym (mapm (fun m : NMap (NMap (value * mem_tag)) => uncurrym m) bufs')).
+
+Record prog :=
+  { procedures : code ;
+    buffers : bufs ;
+  }.
+
+
+
+Definition max_label (p : Intermediate.program) : nat :=
+  let soup := (flatten (flatten (map codomm' (codomm' (Intermediate.prog_procedures p))))) in
+  let get_label i := match i with
+                    | ILabel l => Some l
+                    | _ => None
+                    end in
+  let labels := pmap get_label soup in foldl max 0 labels + 1.
+
+Definition max_proc_id (p : Intermediate.program) : nat :=
+  let componnent_max_proc_id (map : NMap Machine.code) : nat :=
+      foldl max 0 (domm map) in
+  let max_proc_ids := map componnent_max_proc_id (codomm' (Intermediate.prog_procedures p)) in
+  foldl max 0 max_proc_ids + 1.
+
+Definition linearize (p : Intermediate.program) : prog :=
+  let lmax := max_label p in
+  let pmax := max_proc_id p in
+  let cenv := {| program := p ;
+                 make_label := (fun c p => lmax + c * pmax + p) |} in
+  {| procedures := linearize_code_bis cenv ;
+     buffers    := linearize_bufs cenv |}.
+*)
+
+
+(* 
+
+
+Module Compartmentless_Pointer.
+  Definition t : Type := Block.id * Block.offset.
+
+  Definition block (p : t) : Block.id :=
+    let '(b, _) := p in b.
+
+  Definition offset (p : t) : Block.offset :=
+    let '( _, o) := p in o.
+
+  Definition eq (p1 p2 : t) : bool :=
+    let '( b1, o1) := p1 in
+    let '(b2, o2) := p2 in
+ (Nat.eqb b1 b2) && (Z.eqb o1 o2).
+
+  Definition leq (p1 p2 : t) : option bool :=
+    let '(b1, o1) := p1 in
+    let '( b2, o2) := p2 in
+    if  (Nat.eqb b1 b2) then
+      Some ((o1 <=? o2) % Z)
+    else
+      None.
+
+  Definition add (ptr : t) (offset : Z) : t :=
+    let '( b, o) := ptr in (b, (o+offset)%Z).
+
+  Definition sub (ptr : t) (offset : Z) : t :=
+    let '(C, b, o) := ptr in (C, b, (o-offset)%Z).
+
+  Definition inc (ptr : t) : t := add ptr 1.
+
+  Lemma add_preserves_component:
+    forall p n, component (add p n) = component p.
+  Proof.
+    intros p n.
+    destruct p as [[C b] o].
+    reflexivity.
+  Qed.
+
+  Lemma add_preserves_block:
+    forall p n, block (add p n) = block p.
+  Proof.
+    intros p n.
+    destruct p as [[C b] o].
+    reflexivity.
+  Qed.
+
+  Lemma inc_preserves_component:
+    forall p, component (inc p) = component p.
+  Proof.
+    intros p.
+    destruct p as [[C b] o].
+    reflexivity.
+  Qed.
+
+  Lemma inc_preserves_block:
+    forall p, block (inc p) = block p.
+  Proof.
+    intros p.
+    destruct p as [[C b] o].
+    reflexivity.
+  Qed.
+
+  Lemma compose :
+    forall ptr,
+      (component ptr, block ptr, offset ptr) = ptr.
+  Proof.
+    now intros [[C b] o].
+  Qed.
+End Pointer.
+
+
+*)
